Add an invariant for INSTREAM_BUFFERED_def

basis/TextIOProofScript.sml
@@ -564,19 +564,36 @@ val REF_NUM_def = Define `
   REF_NUM loc n =
     SEP_EXISTS v. REF loc v * & (NUM n v)`;
 
-val REF_BOOL_def = Define `
-  REF_BOOL loc b =
-    SEP_EXISTS bv. REF loc bv * & (BOOL b bv)`;
+val instream_buffered_inv_def = Define `
+  instream_buffered_inv r w fs fd bcontent content =
+    ?pos.
+      get_file_content fs fd = SOME (content,pos) /\
+      r < LENGTH bcontent /\
+      w < LENGTH bcontent /\
+      ~(r>w) /\
+      bcontent = TAKE (w-r) (DROP (pos-(w-r)) (MAP (n2w o ORD) content))`;
 
 val INSTREAM_BUFFERED_def = Define `
-  INSTREAM_BUFFERED is =
-    SEP_EXISTS ir i jr j full fullv buff content fd fdv.
-      & (is = (Conv (SOME (TypeStamp "InstreamBuffered" 9)) [fdv; ir; jr; buff; full])) *
+  INSTREAM_BUFFERED fs fd  is =
+    SEP_EXISTS rr r wr w buff bcontent fdv.
+      & (is = (Conv (SOME (TypeStamp "InstreamBuffered" 11)) [fdv; rr; wr; buff])) *
       & (INSTREAM fd fdv) *
-      REF_NUM ir i *
-      REF_NUM jr j *
-      W8ARRAY buff content *
-      REF_BOOL full fullv`;
+      & (instream_buffered_inv r w fs fd bcontent) *
+      STDIO fs *
+      REF_NUM rr r *
+      REF_NUM wr w *
+      W8ARRAY buff bcontent`;
+
+val INSTREAM_BUFFERED_def = Define `
+  INSTREAM_BUFFERED fs fd r w is =
+    SEP_EXISTS rr wr buff bcontent fdv.
+      & (is = (Conv (SOME (TypeStamp "InstreamBuffered" 11)) [fdv; rr; wr; buff])) *
+      & (INSTREAM fd fdv) *
+      & (instream_buffered_inv r w fs fd bcontent) *
+      STDIO fs *
+      REF_NUM rr r *
+      REF_NUM wr w *
+      W8ARRAY buff bcontent`;
 
 val OUTSTREAM_def = Define `
   OUTSTREAM fd fdv <=>
@@ -1675,6 +1692,58 @@ Theorem input_spec
   \\ simp[fsupdate_def]
   \\ fs[get_file_content_def]
   \\ xsimpl);
+
+(*
+Theorem b_input_aux1_spec
+  `!fd fdv fs off offv len lenv buf bufv is iswr isrr isbuf isbufv.
+    len + off <= LENGTH buf ∧ len <= w - r /\
+    NUM off offv ∧ NUM len lenv /\
+    is = (Conv (SOME (TypeStamp "InstreamBuffered" 11)) [fdv; rr; wr; isbuff]) /\
+    get_file_content fs fd = SOME(content, pos) ==>
+    get_mode fs fd = SOME ReadMode ==>
+    app (p:'ffi ffi_proj) TextIO_b_input_aux1_v [is; bufv; offv; lenv]
+    (STDIO fs * W8ARRAY bufv buf * INSTREAM_BUFFERED_R_W is r w)
+    (POSTv nv. SEP_EXISTS content. &(NUM (MIN len (LENGTH content-pos)) nv) *
+       W8ARRAY bufv (insert_atI (TAKE len content)
+                                 off buf) *
+        STDIO fs * INSTREAM_BUFFERED is)`
+  (xcf_with_def "TextIO.b_input_aux1" TextIO_b_input_aux1_v_def
+  \\rw[STDIO_def,INSTREAM_BUFFERED_def, INSTREAM_BUFFERED_R_W_def, REF_NUM_def]
+  \\ xpull
+  \\ xmatch
+  \\ xlet_auto >- xsimpl
+  \\ fs[instream_buffered_inv_def]
+  \\ xlet_auto >- (xsimpl >- fs[LENGTH_TAKE])
+  \\ xlet_auto >- xsimpl
+  \\ xlet_auto >- xsimpl
+  \\ xvar \\ xsimpl \\ fs[PULL_EXISTS]
+  \\ map_every qexists_tac [`bcontent`, `r`,`w`, `fd'`,`ll`,`content`,`pos`]
+  \\ xsimpl
+  \\ rw[]
+
+  )
+
+  (
+  \\ `fd = 1 ∨ fd = 2 ⇒ pos = LENGTH content`
+  by (
+    fs[STD_streams_def]
+    \\ fs[get_file_content_def]
+    \\ pairarg_tac \\ fs[]
+    \\ rpt(first_x_assum(qspec_then`fd`mp_tac))
+    \\ rw[] \\ fs[]
+    \\ metis_tac[SOME_11] )
+  \\ `pos = LENGTH content ⇒ MIN (len + pos) (MAX pos (LENGTH content)) = LENGTH content` by simp[MAX_DEF,MIN_DEF]
+  \\ simp[STD_streams_fsupdate]
+  \\ xapp
+  \\ mp_tac(SYM (SPEC_ALL get_file_content_numchars)) \\ rw[]
+  \\ mp_tac(get_mode_with_numchars) \\ rw[]
+  \\ instantiate \\ xsimpl
+  \\ simp[fsupdate_numchars] \\ rw[]
+  \\ qexists_tac`THE (LDROP x ll)`
+  \\ simp[fsupdate_def]
+  \\ fs[get_file_content_def]
+  \\ xsimpl);
+*)
 
 Theorem extend_array_spec
     `∀arrv arr.
